CopyPropagation.v
@@ -1,7 +1,7 @@
 Require Import CSet Le.
 
 Require Import Plus Util AllInRel Map.
-Require Import Val Var Env EnvTy IL Sim Coherence Fresh Annotation DecSolve SetOperations LabelsDefined.
+Require Import Val Var Env IL Sim Coherence Fresh Annotation DecSolve SetOperations LabelsDefined.
 
 Require Import Liveness Eqn ValueOpts RenamedApart.
 
