GVN.v
@@ -1,7 +1,7 @@
 Require Import CSet Le.
 
 Require Import Plus Util AllInRel Map.
-Require Import CSet Val Var Env EnvTy IL Sim Alpha Coherence Fresh Annotation MoreExp.
+Require Import CSet Val Var Env IL Sim Alpha Coherence Fresh Annotation MoreExp.
 
 Require Import Liveness Filter.
 
